Prove `cyes` is `data_safe`
* `cyes` prints its character argument in a loop and
  does not terminate

examples/cost/divProgScript.sml
@@ -131,7 +131,7 @@ fun mk_code_lookup code_tm code_def = EVERY_lookup
 (* remove makespace bindings *)
 val strip_makespace =
   qmatch_goalsub_abbrev_tac `bind _ rest_mkspc _`
-  \\ REWRITE_TAC [ bind_def, makespace_def ]
+  \\ REWRITE_TAC [ bind_def, makespace_def, add_space_def]
   \\ eval_goalsub_tac ``cut_env _ _`` \\ simp []
   \\ eval_goalsub_tac ``state_locals_fupd _ _``
   \\ Q.UNABBREV_TAC `rest_mkspc`
@@ -144,6 +144,7 @@ fun mk_strip_assign code_lookup =
                  , do_app_def         , data_spaceTheory.op_space_req_def
                  , do_space_def       , closLangTheory.op_distinct
                  , MEM                , IS_NONE_DEF
+                 , add_space_def      , check_lim_def
                  , bvi_to_dataTheory.op_requires_names_eqn ]
   \\ BETA_TAC
   \\ TRY(eval_goalsub_tac ``cut_state _ _`` \\ simp [])
@@ -224,7 +225,6 @@ val make_if =
                  , backend_commonTheory.false_tag_def]
   \\ simp [pop_env_def]
   \\ eval_goalsub_tac ``state_locals_fupd _ _``
-
 
 (* ************ *)
 (* * pureLoop * *)
@@ -489,7 +489,7 @@ end
 QED
 
 (* ************************** *)
-(* * echo (with mini-basis) * *)
+(* * cyes (with mini-basis) * *)
 (* ************************** *)
 
 val word8_mod =
@@ -510,7 +510,7 @@ val word8array_mod =
 val word8array_array =
   find_term (can (match_term ``Dlet _ (Pvar "array") _``)) word8array_mod
 
-val echo =
+val cyes =
   let val prog = process_topdecs `
       fun put_char c = let
         val s = String.implode [c]
@@ -527,7 +527,7 @@ val echo =
                             ] ++ ^prog``
   end
 
-val echo2 =
+val cyes2 =
   let val prog = process_topdecs `
       fun put_char c = let
         val a = Word8Array.array 0 (Word8.fromInt 0)
@@ -544,29 +544,347 @@ val echo2 =
                             ] ++ ^prog``
   end
 
-val (echo_call_def,echo_code_def) =
-  to_data echo "echo"
+val (cyes_call_def,cyes_code_def) =
+  to_data cyes "cyes"
 
-val (echo2_call_def,echo2_code_def) =
-  to_data echo2 "echo2"
+val (cyes2_call_def,cyes2_code_def) =
+  to_data cyes2 "cyes2"
 
-val f_diff = diff_codes echo_code_def echo2_code_def
+val f_diff = diff_codes cyes_code_def cyes2_code_def
 
 val (f11,f12) = hd f_diff
 val (f21,f22) = (hd o tl) f_diff
 
-Theorem data_safe_echo_code:
+Theorem size_of_Number_head:
+  ∀vs refs seen n. size_of (Number n::vs) refs seen = size_of vs refs seen
+Proof
+  Cases \\ rw [size_of_def] \\ pairarg_tac \\ fs []
+QED
+
+Theorem size_of_seen_SUBSET:
+  ∀vs refs seen n1 seen1 refs1.
+  (size_of vs refs seen = (n1,refs1,seen1))
+  ⇒ domain seen ⊆  domain seen1
+Proof
+  ho_match_mp_tac size_of_ind \\ rw [size_of_def]
+  \\ rpt (pairarg_tac \\ fs []) \\ rveq
+  >- (ho_match_mp_tac SUBSET_TRANS
+     \\ asm_exists_tac \\ fs [])
+ \\ every_case_tac \\ fs []
+ \\ first_x_assum irule
+ \\ rpt (pairarg_tac \\ fs [])
+QED
+
+Theorem size_of_le_head:
+  ∀vs refs seen v n1 seen1 refs1 n2 refs2 seen2.
+   (size_of (v::vs) refs seen = (n1,refs1,seen1)) ∧
+   (size_of vs refs seen = (n2,refs2,seen2))
+   ⇒ n2 ≤ n1
+Proof
+  Cases \\ fs [size_of_def]
+  \\ rw [] \\ rpt (pairarg_tac \\ fs []) \\ rveq
+QED
+
+Theorem size_of_le_APPEND:
+  ∀a b refs seen n1 seen1 refs1 n2 refs2 seen2.
+   (size_of (a ++ b) refs seen = (n1,refs1,seen1)) ∧
+   (size_of b refs seen = (n2,refs2,seen2))
+   ⇒ n2 ≤ n1
+Proof
+  Induct
+  >- (rw [] \\ fs [])
+  \\ rw [] \\ irule LESS_EQ_TRANS
+  \\ qexists_tac `FST (size_of (a++b) refs seen)`
+  \\ Cases_on `size_of (a++b) refs seen` \\ Cases_on `r`
+  \\ simp []
+  \\ conj_tac
+  >- (first_x_assum irule \\ metis_tac [])
+  \\ (ho_match_mp_tac size_of_le_head \\ metis_tac [])
+QED
+
+Definition closed_ptrs_list_def:
+  (closed_ptrs_list [] refs = T)
+∧ (closed_ptrs_list (RefPtr p::vs) refs =
+     IS_SOME (lookup p refs) ∧
+     closed_ptrs_list vs refs)
+∧ (closed_ptrs_list (Block ts tag l::vs) refs =
+     closed_ptrs_list l refs ∧
+     closed_ptrs_list vs refs)
+∧ (closed_ptrs_list (v::vs) refs = closed_ptrs_list vs refs)
+Termination
+  WF_REL_TAC `(inv_image (measure v1_size) (\(vs,refs). vs))`
+End
+
+
+Definition closed_ptrs_refs_def:
+  closed_ptrs_refs refs =
+    ∀x l. (sptree$lookup x refs = SOME (ValueArray l))
+        ⇒ closed_ptrs_list l refs
+End
+
+Definition closed_ptrs_def:
+  closed_ptrs vs refs = closed_ptrs_list vs refs ∧ closed_ptrs_refs refs
+End
+
+Theorem closed_ptrs_cons_intro:
+  ∀vs refs v. closed_ptrs (v::vs) refs ⇒ closed_ptrs vs refs ∧ closed_ptrs [v] refs
+Proof
+  ho_match_mp_tac closed_ptrs_list_ind
+  \\ rw [closed_ptrs_def,closed_ptrs_list_def]
+  \\ Cases_on `v` \\ fs [closed_ptrs_list_def]
+QED
+
+Theorem closed_ptrs_cons_dest:
+  ∀vs refs v. closed_ptrs vs refs ∧ closed_ptrs [v] refs ⇒ closed_ptrs (v::vs) refs
+Proof
+  ho_match_mp_tac closed_ptrs_list_ind
+  \\ rw [closed_ptrs_def,closed_ptrs_list_def]
+  \\ Cases_on `v` \\ fs [closed_ptrs_list_def]
+QED
+
+Theorem closed_ptrs_cons:
+  ∀vs refs v. closed_ptrs (v::vs) refs = closed_ptrs vs refs ∧ closed_ptrs [v] refs
+Proof
+  rw [] \\ eq_tac \\ fs [closed_ptrs_cons_dest]
+  \\ rw [] \\ drule closed_ptrs_cons_intro \\ rw []
+QED
+
+Definition live_ptr_list_def:
+  (live_ptr_list p [] = F)
+∧ (live_ptr_list p (RefPtr n::vs) = ((p = n) ∨ live_ptr_list p vs))
+∧ (live_ptr_list p (Block ts tag l::vs) = (live_ptr_list p l ∨ live_ptr_list p vs))
+∧ (live_ptr_list p (v::vs) = live_ptr_list p vs)
+Termination
+  WF_REL_TAC `(inv_image (measure v1_size) (\(p,vs). vs))`
+End
+
+Definition live_ptr_def:
+  (live_ptr p vs refs =
+     live_ptr_list p vs ∨
+     (∃x l. (sptree$lookup x refs = SOME (ValueArray l)) ∧
+            live_ptr_list p l))
+End
+
+Theorem live_ptr_cons:
+  ∀p vs refs v. live_ptr p (v::vs) refs = live_ptr p [v] refs ∨ live_ptr p vs refs
+Proof
+  ho_match_mp_tac live_ptr_list_ind \\ rw [live_ptr_def,live_ptr_list_def]
+  \\ EQ_TAC \\ rw []
+  \\ TRY (Cases_on `v` \\ fs [live_ptr_list_def] \\ NO_TAC)
+  \\ metis_tac []
+QED
+
+Theorem size_of_refs_subspt:
+  ∀vs refs seen n refs' seen'.
+    (size_of vs refs seen = (n,refs',seen'))
+    ⇒ subspt refs' refs
+Proof
+  ho_match_mp_tac size_of_ind \\ rw [size_of_def]
+  \\ rpt (pairarg_tac \\ fs []) \\ rveq
+  >- (irule subspt_trans \\ metis_tac [])
+  \\ EVERY_CASE_TAC \\ fs []
+  \\ rpt (pairarg_tac \\ fs []) \\ rveq
+  \\ fs [subspt_delete] \\ irule subspt_trans
+  \\ asm_exists_tac \\ fs [subspt_delete]
+QED
+
+Theorem not_live_ptr_subspt:
+  ∀vs refs refs' p.
+    subspt refs' refs ∧
+    ¬live_ptr p vs refs
+    ⇒¬live_ptr p vs refs'
+Proof
+  rw [live_ptr_def] \\ fs []
+  \\ first_x_assum (qspecl_then [`x`,`l`] assume_tac) \\ rw []
+  >- (disj1_tac \\ CCONTR_TAC \\ fs [subspt_lookup]
+     \\ first_x_assum drule \\ rw [])
+  \\ disj2_tac \\ rw []
+QED
+
+Theorem live_ptr_ptr:
+  ∀r refs l p.
+   (lookup r refs = SOME (ValueArray l))
+   ⇒ (live_ptr p [RefPtr r] refs = ((p = r) ∨ live_ptr p l refs))
+Proof
+  rw [] \\ EQ_TAC
+  \\ rw [live_ptr_def] \\ fs [live_ptr_list_def]
+  \\ metis_tac []
+QED
+
+Theorem live_ptr_delete:
+  ∀vs p refs r l.
+    p ≠ r ∧ (lookup r refs = SOME (ValueArray l))
+    ⇒ (live_ptr p vs refs = live_ptr_list p l ∨ live_ptr p vs (delete r refs))
+Proof
+  rw []
+  \\ EQ_TAC \\ rw [live_ptr_def] \\ fs [live_ptr_list_def]
+  >- (Cases_on `x = r` \\ fs [] \\ rveq \\ metis_tac [lookup_delete])
+  >- metis_tac []
+  \\ Cases_on `x = r` \\ fs [lookup_delete] \\ metis_tac [lookup_delete]
+QED
+
+Theorem insert_delete_swap:
+  ∀k v x r.
+   wf r ∧ k ≠ x
+   ⇒ (insert k v (delete x r) = delete x (insert k v r))
+Proof
+  rw []
+  \\ `wf (insert k v (delete x r))` by rw [wf_insert,wf_delete]
+  \\ `wf (delete x (insert k v r))` by rw [wf_insert,wf_delete]
+  \\ drule spt_eq_thm \\ disch_then (qspec_then `insert k v (delete x r)` drule)
+  \\ rw [] \\ rw [lookup_delete,lookup_insert]
+QED
+
+Theorem wf_size_of:
+  ∀vs refs seen n' refs' seen'.
+    wf refs ∧ (size_of vs refs seen = (n',refs',seen'))
+    ⇒ wf refs'
+Proof
+  ho_match_mp_tac size_of_ind \\ rw [size_of_def] \\ fs []
+  \\ rpt (pairarg_tac \\ fs []) \\ rveq
+  \\ every_case_tac \\ fs []
+  \\ rpt (pairarg_tac \\ fs []) \\ rveq
+  \\ fs [wf_delete]
+QED
+
+Triviality size_of_insert_aux:
+  ∀vs refs seen p x n refs' seen'.
+    wf refs                 ∧
+    ¬live_ptr p vs refs     ∧
+    (lookup p refs = NONE)  ∧
+    (size_of vs refs seen = (n,refs',seen'))
+    ⇒ (size_of vs (insert p x refs) seen = (n,insert p x refs',seen'))
+Proof
+  ho_match_mp_tac size_of_ind \\ rw [size_of_def]
+  \\ rpt (pairarg_tac \\ fs []) \\ rveq
+  >- (qpat_x_assum `¬ _` (assume_tac o ONCE_REWRITE_RULE [live_ptr_cons])
+     \\ fs [] \\ first_x_assum drule
+     \\ disch_then (qspec_then `x'` assume_tac) \\ rfs [] \\ rveq
+     \\ `subspt refs1' refs` by
+        (ho_match_mp_tac size_of_refs_subspt
+        \\ asm_exists_tac \\ fs [])
+     \\ drule wf_size_of \\ disch_then (drule_then assume_tac)
+     \\ drule_then (qspec_then `[x]` (drule_then assume_tac)) not_live_ptr_subspt
+     \\ first_x_assum (drule_then (drule_then (qspec_then `x'` mp_tac)))
+     \\ impl_tac
+     >- (CCONTR_TAC \\ fs []
+        \\ Cases_on `lookup p refs1'`
+        \\ fs [subspt_lookup]
+        \\ first_x_assum drule \\ fs [])
+     \\ rw [])
+  >- (`p ≠ r` by fs [live_ptr_def,live_ptr_list_def]
+     \\ fs [lookup_insert]
+     \\ every_case_tac \\ fs [] \\ rveq
+     >- (rpt (pairarg_tac \\ fs []) \\ rveq
+        \\ drule live_ptr_ptr
+        \\ disch_then (qspec_then `p` (fn t => fs [t]))
+        \\ drule live_ptr_delete
+        \\ disch_then (drule_then (qspec_then `l` (fn t => fs [t])))
+        \\ drule_then (qspec_then `r` assume_tac) wf_delete
+        \\ first_x_assum drule \\ disch_then drule \\ fs [lookup_delete]
+        \\ disch_then (qspec_then `x` assume_tac) \\ fs []
+        \\ qpat_x_assum `_ = (_,refs'',seen'')` mp_tac
+        \\ qmatch_goalsub_abbrev_tac `size_of l refs1 seen`
+        \\ qmatch_asmsub_abbrev_tac  `size_of l refs2 seen`
+        \\ `refs1 = refs2` suffices_by fs []
+        \\ UNABBREV_ALL_TAC \\ fs [insert_delete_swap])
+     \\ fs [insert_delete_swap])
+  \\ fs [live_ptr_def,live_ptr_list_def]
+  \\ first_x_assum drule \\ disch_then drule \\ disch_then drule
+  \\ disch_then (qspec_then `x` assume_tac) \\ fs [] \\ rfs []
+QED
+
+Theorem closed_ptrs_list_not_live_ptr_list:
+  ∀p vs refs.
+    closed_ptrs_list vs refs ∧
+    (lookup p refs = NONE)
+    ⇒ ¬live_ptr_list p vs
+Proof
+  ho_match_mp_tac live_ptr_list_ind\\ rw [closed_ptrs_list_def,live_ptr_list_def]
+  \\ fs [IS_SOME_EXISTS]
+  >- (CCONTR_TAC \\ fs [])
+  \\ first_x_assum ho_match_mp_tac \\ metis_tac []
+QED
+
+Theorem closed_ptrs_not_live_ptr:
+  ∀vs refs p.
+    closed_ptrs vs refs ∧
+    (lookup p refs = NONE)
+    ⇒ ¬live_ptr p vs refs
+Proof
+  rw [closed_ptrs_def,live_ptr_def]
+  >- (drule closed_ptrs_list_not_live_ptr_list \\ disch_then drule \\ fs [])
+  \\ CCONTR_TAC \\ fs [closed_ptrs_refs_def]  \\ first_x_assum drule \\ strip_tac
+  \\ drule closed_ptrs_list_not_live_ptr_list \\ disch_then drule \\ fs []
+QED
+
+Theorem size_of_insert:
+  ∀vs refs seen p x n refs' seen'.
+    wf refs                 ∧
+    closed_ptrs vs refs     ∧
+    (lookup p refs = NONE)  ∧
+    (size_of vs refs seen = (n,refs',seen'))
+    ⇒ (size_of vs (insert p x refs) seen = (n,insert p x refs',seen'))
+Proof
+  rw [] \\ ho_match_mp_tac size_of_insert_aux
+  \\ fs [closed_ptrs_not_live_ptr]
+QED
+
+Theorem closed_ptrs_APPEND:
+  ∀a b refs. closed_ptrs (a ++ b) refs = closed_ptrs a refs ∧ closed_ptrs b refs
+Proof
+  Induct
+  >- (rw [closed_ptrs_def,closed_ptrs_list_def] \\ metis_tac [])
+  \\ rw [] \\ ONCE_REWRITE_TAC [closed_ptrs_cons] \\ metis_tac []
+QED
+
+Theorem closed_ptrs_refs_insert:
+  ∀refs p x y.
+    closed_ptrs_refs refs ∧
+    (lookup p refs = NONE)
+    ⇒ closed_ptrs_refs (insert p (ByteArray x y) refs)
+Proof
+  rw [closed_ptrs_refs_def]
+  \\ Cases_on `x' = p` \\ fs [lookup_insert]
+  \\ first_x_assum drule
+  \\ pop_assum kall_tac
+  \\ pop_assum kall_tac
+  \\ pop_assum mp_tac
+  \\ Q.SPEC_TAC (`refs`,`refs`)
+  \\ Q.SPEC_TAC (`l`,`l`)
+  \\ ho_match_mp_tac closed_ptrs_list_ind
+  \\ rw [closed_ptrs_list_def]
+  \\ metis_tac [IS_SOME_EXISTS,lookup_insert]
+QED
+
+Theorem closed_ptrs_insert:
+  ∀vs refs p x.
+  closed_ptrs vs refs
+  ∧ (lookup p refs = NONE)
+  ∧ closed_ptrs_refs (insert p x refs)
+  ⇒ closed_ptrs vs (insert p x refs)
+Proof
+  ho_match_mp_tac closed_ptrs_list_ind
+  \\ rw [closed_ptrs_def]
+  \\ fs [closed_ptrs_list_def]
+  \\ metis_tac [lookup_insert,IS_SOME_EXISTS]
+QED
+
+Theorem data_safe_cyes_code:
   ∀s ts.
    s.safe_for_space ∧
-   check_state s ∧
-   size_of_heap s ≤ s.limits.heap_limit ∧
+   wf s.refs ∧
+   closed_ptrs (stack_to_vs s) s.refs ∧
+   size_of_heap s + 4 ≤ s.limits.heap_limit ∧
+   2 ≤ s.limits.length_limit ∧
    (s.tstamps = SOME ts) ∧
-   (∃x. lookup 0 s.locals = SOME (Number 97)) ∧
-   (s.code = echo_data_code)
+   0 < ts ∧
+   (lookup 0 s.locals = SOME (Number 97)) ∧
+   (s.code = cyes_data_code)
    ⇒ data_safe (evaluate ((SND o SND) ^f21, s))
 Proof
   let
-    val code_lookup   = mk_code_lookup `echo_data_code` echo_code_def
+    val code_lookup   = mk_code_lookup `cyes_data_code` cyes_code_def
     val strip_assign  = mk_strip_assign code_lookup
     val open_call     = mk_open_call code_lookup
     val make_call     = mk_make_call open_call
@@ -580,49 +898,462 @@ Proof
         , initial_state_def ]
   \\ rw []
   \\ strip_call
-  \\ qmatch_goalsub_abbrev_tac `f (state_locals_fupd _ _)`
-  \\ qmatch_goalsub_abbrev_tac `f s1`
-  \\ Q.UNABBREV_TAC `f`
-  \\ `check_state s1` by
-     by (Q.UNABBREV_TAC `s1`
-        \\ rw [check_state_def]
-        >- EVAL_TAC
-        >-
-
-
-  \\ strip_makespace
-  \\ ntac 6 strip_assign
-  \\ strip_call
-
-
-``lookup 61 echo_data_code``
-|> (REWRITE_CONV [echo_code_def] THENC EVAL)
-(* Finds out the length of the array *)
-
-``lookup 62 echo_data_code``
-|> (REWRITE_CONV [echo_code_def] THENC EVAL)
-(* Move the string into a byte array *)
-
-
-  \\ rw [ evaluate_def,get_var_def
-        , lookup_fromAList,get_vars_def
-        , find_code_def,call_env_def,data_safe_def]
-  \\ rw [lookup_fromList,dec_clock_def,lookup_fromAList,data_safe_def,cut_env_def]
-  \\ qmatch_goalsub_abbrev_tac `evaluate (_,s')`
-  \\ `s'.clock < s.clock` by rw [Abbr `s'`]
-
-
+  \\ `toListA [] (inter s.locals (LS ())) = [Number 97]`
+     by (Cases_on `s.locals` \\ fs [lookup_def,inter_def,toListA_def])
+  (* strip_makespace *)
+  \\ qmatch_goalsub_abbrev_tac `bind _ rest_mkspc _`
+  \\ REWRITE_TAC [ bind_def, makespace_def, add_space_def]
+  \\ `cut_env (LS ()) s.locals = SOME (LS (Number 97))`
+     by (REWRITE_TAC [cut_env_def,domain_def,SUBSET_DEF]
+        \\ fs [domain_lookup] \\ Cases_on `s.locals`
+        \\ fs [lookup_def,inter_def,toListA_def])
+  \\ simp []
+  \\ Q.UNABBREV_TAC `rest_mkspc`
+  \\ eval_goalsub_tac ``cut_env _ _`` \\ simp []
+  (* strip_assign *)
+  \\ `2 < 2 ** s.limits.length_limit`
+     by (Cases_on `s.limits.length_limit` \\ fs [])
+  \\ ntac 2 strip_assign
+  \\ strip_assign \\ fs []
+  \\ ntac 3 (strip_assign \\ fs [])
+  \\ eval_goalsub_tac ``state_locals_fupd _ _``
+  (* strip_call *)
+  \\ qmatch_goalsub_abbrev_tac (`bind _ rest_call2 _`)
+  \\ ONCE_REWRITE_TAC [bind_def]
+  \\ ASM_REWRITE_TAC [ call_def     , find_code_def , push_env_def
+                     , get_vars_def , call_env_def  , dec_clock_def
+                     , cut_env_def  , domain_def    , data_safe_def
+                     , EMPTY_SUBSET , get_var_def ]
+  \\ simp [code_lookup,lookup_def,domain_IS_SOME]
+  (* Prove we are safe for space up to this point *)
+  \\ qmatch_goalsub_abbrev_tac `state_safe_for_space_fupd (K safe)  _`
+  \\ `safe` by
+     (Q.UNABBREV_TAC `safe`
+     \\ simp [data_safe_def,size_of_def,size_of_Number_head]
+     \\ fs [size_of_heap_def,stack_to_vs_def]
+     \\ rpt (pairarg_tac \\ fs []) \\ rveq
+     \\ `n ≤ n'` by
+        (irule size_of_le_APPEND
+        \\ asm_exists_tac \\ fs []
+        \\ asm_exists_tac \\ fs [])
+     \\ irule LESS_EQ_TRANS \\ qexists_tac `n' + 3` \\ rw [])
+  \\ simp []
+  \\ Q.UNABBREV_TAC `safe`
+  \\ IF_CASES_TAC >- simp [data_safe_def]
+  \\ REWRITE_TAC [ push_env_def , to_shallow_def , to_shallow_thm]
+  \\ eval_goalsub_tac ``state_locals_fupd _ _``
+  (* strip_assign *)
+  \\ strip_assign
+  \\ make_if
+  \\ ntac 4 strip_assign
+  (* open_tailcall *)
+  \\ ASM_REWRITE_TAC [ tailcall_def , find_code_def
+                     , get_vars_def , get_var_def
+                     , lookup_def   , timeout_def ]
+  \\ simp [code_lookup,lookup_def]
+  (* Prove we are safe for space up to this point *)
+  \\ qmatch_goalsub_abbrev_tac `state_safe_for_space_fupd (K safe)  _`
+  \\ `safe` by
+     (Q.UNABBREV_TAC `safe`
+     \\ simp [data_safe_def,size_of_def,size_of_Number_head]
+     \\ fs [size_of_heap_def,stack_to_vs_def]
+     \\ rpt (pairarg_tac \\ fs []) \\ rveq
+     \\ Cases_on `ts` \\ fs [size_of_def,lookup_def]
+     \\ `n1''''' ≤ n''` by
+        (irule size_of_le_APPEND
+        \\ asm_exists_tac \\ fs []
+        \\ asm_exists_tac \\ fs [])
+     \\ Cases_on `lookup (SUC n) seen1'''''` \\ fs [] \\ rveq \\ fs [])
+  \\ simp []
+  \\ Q.UNABBREV_TAC `safe`
+  \\ IF_CASES_TAC >- simp [data_safe_def]
+  \\ REWRITE_TAC [ call_env_def   , dec_clock_def
+                 , to_shallow_thm , to_shallow_def ]
+  \\ eval_goalsub_tac ``state_locals_fupd _ _``
+  \\ strip_assign
+  \\ make_if
+  \\ Q.UNABBREV_TAC `rest_call2`
+  (* strip_assign *)
+  \\ strip_assign
+  \\ Q.ABBREV_TAC `pred = ∃w. 0 = w2n (w:word8)`
+  \\ `pred` by (UNABBREV_ALL_TAC \\ qexists_tac `n2w 0` \\ rw [])
+  \\ fs [] \\ pop_assum kall_tac \\ pop_assum kall_tac
+  \\ eval_goalsub_tac ``state_locals_fupd _ _``
+  (* strip_call *)
+  \\ qmatch_goalsub_abbrev_tac (`bind _ rest_call2 _`)
+  \\ ONCE_REWRITE_TAC [bind_def]
+  \\ ASM_REWRITE_TAC [ call_def     , find_code_def , push_env_def
+                     , get_vars_def , call_env_def  , dec_clock_def
+                     , cut_env_def  , domain_def    , data_safe_def
+                     , EMPTY_SUBSET , get_var_def ]
+  \\ simp [code_lookup,lookup_def,domain_IS_SOME]
+  (* Prove we are safe for space up to this point *)
+  \\ qmatch_goalsub_abbrev_tac `state_safe_for_space_fupd (K safe)  _`
+  \\ `safe` by
+     (Q.UNABBREV_TAC `safe`
+     \\ simp [data_safe_def,size_of_def,size_of_Number_head]
+     \\ fs [size_of_heap_def,stack_to_vs_def,size_of_Number_head]
+     \\ rpt (pairarg_tac \\ fs []) \\ rveq
+     \\ Cases_on `ts` \\ fs [size_of_def,lookup_def]
+     \\ rpt (pairarg_tac \\ fs []) \\ rveq
+     \\ fs [size_of_Number_head] \\ rveq
+     \\ Cases_on `lookup (SUC n) seen1'''''` \\ fs [])
+  \\ simp [] \\ Q.UNABBREV_TAC `safe`
+  \\ IF_CASES_TAC >- simp [data_safe_def]
+  \\ REWRITE_TAC [ push_env_def , to_shallow_def , to_shallow_thm]
+  \\ eval_goalsub_tac ``state_locals_fupd _ _``
+  (* strip_assign *)
+  \\ strip_assign
+  \\ make_if
+  \\ ntac 3 strip_assign
+  \\ Q.ABBREV_TAC `pred = ∃w. 97 = w2n (w:word8)`
+  \\ `pred` by (UNABBREV_ALL_TAC \\ qexists_tac `n2w 97` \\ rw [])
+  \\ fs [] \\ pop_assum kall_tac \\ pop_assum kall_tac
+  \\ ntac 4 strip_assign
+  (* make_tailcall *)
+  \\ ASM_REWRITE_TAC [ tailcall_def , find_code_def
+                     , get_vars_def , get_var_def
+                     , lookup_def   , timeout_def ]
+  \\ simp [code_lookup,lookup_def]
+  \\ fs [insert_shadow]
+  \\ qmatch_goalsub_abbrev_tac `insert p1 _ s.refs`
+  \\ `lookup p1 s.refs = NONE` by
+     (Q.UNABBREV_TAC `p1` \\ fs [least_from_def]
+     \\ EVERY_CASE_TAC \\ fs [] \\ numLib.LEAST_ELIM_TAC
+     >- metis_tac []
+     \\ mp_then Any assume_tac IN_INFINITE_NOT_FINITE INFINITE_NUM_UNIV
+     \\ rw [] \\ pop_assum (qspec_then `domain s.refs` assume_tac)
+     \\ fs [FINITE_domain,domain_lookup]
+     \\ Cases_on `lookup x s.refs` \\ fs []
+     \\ asm_exists_tac \\ fs [])
+  \\ qmatch_goalsub_abbrev_tac `state_safe_for_space_fupd (K safe)  _`
+  \\ `safe` by
+     (Q.UNABBREV_TAC `safe`
+     \\ simp [data_safe_def,size_of_def,size_of_Number_head]
+     \\ fs [size_of_heap_def,stack_to_vs_def,size_of_Number_head]
+     \\ rpt (pairarg_tac \\ fs []) \\ rveq
+     \\ fs [size_of_Number_head,insert_shadow] \\ rveq
+     \\ qmatch_asmsub_abbrev_tac `closed_ptrs (a ++ b ++ c)`
+     \\ `closed_ptrs (b ++ c) s.refs` by fs [closed_ptrs_APPEND]
+     \\ map_every  Q.UNABBREV_TAC [`a`,`b`,`c`]
+     \\ drule size_of_insert \\ disch_then drule
+     \\ disch_then (qspecl_then [`LN`,`p1`] mp_tac)
+     \\ qmatch_asmsub_abbrev_tac `insert p1 x s.refs`
+     \\ disch_then drule \\ disch_then (drule_then (qspec_then `x` assume_tac))
+     \\ fs [] \\ rveq \\ rfs []
+     \\ Q.UNABBREV_TAC `x` \\ fs [])
+  \\ simp [] \\ Q.UNABBREV_TAC `safe`
+  \\ IF_CASES_TAC >- simp [data_safe_def]
+  \\ REWRITE_TAC [ call_env_def   , dec_clock_def
+                 , to_shallow_thm , to_shallow_def ]
+  \\ eval_goalsub_tac ``state_locals_fupd _ _``
+  \\ strip_assign
+  \\ make_if
+  \\ Q.UNABBREV_TAC `rest_call2`
+  \\ strip_assign
+  \\ strip_assign
+  \\ strip_assign
+  \\ Q.ABBREV_TAC `pred = ∃w. 0 = w2n (w:word8)`
+  \\ `pred` by (UNABBREV_ALL_TAC \\ qexists_tac `n2w 0` \\ rw [])
+  \\ fs [] \\ pop_assum kall_tac \\ pop_assum kall_tac
+  \\ eval_goalsub_tac ``state_locals_fupd _ _``
+  \\ qmatch_goalsub_abbrev_tac `insert p2 _ (insert p1 _ s.refs)`
+  \\ strip_assign
+  \\ fs [lookup_insert]
+  \\ `p1 ≠ p2` by
+     (rw [Abbr `p2`,least_from_def]
+     >- (CCONTR_TAC \\ fs [])
+     >- (numLib.LEAST_ELIM_TAC \\ rw []
+        \\ Cases_on `ptr = p1` \\ fs []
+        \\ qexists_tac `ptr` \\ fs [])
+     \\ numLib.LEAST_ELIM_TAC \\ rw [] \\ fs []
+     \\ mp_then Any assume_tac IN_INFINITE_NOT_FINITE INFINITE_NUM_UNIV
+     \\ rw [] \\ pop_assum (qspec_then `domain (insert p1 ARB s.refs)` assume_tac)
+     \\ fs [FINITE_domain,domain_lookup] \\ Cases_on `lookup x (insert p1 ARB s.refs)`
+     \\ fs [] \\ qexists_tac `x` \\ Cases_on `x = p1` \\ fs [lookup_insert])
+  \\ fs []
+  \\ `lookup p2 (insert p1 (ByteArray T [97w]) s.refs) = NONE` by
+     (fs [lookup_insert]
+     \\ rw [Abbr `p2`, least_from_def]
+     >- (Cases_on `p1 = 0` \\ fs [])
+     >- (numLib.LEAST_ELIM_TAC \\ rw []
+        \\ Cases_on `ptr = p1` \\ fs []
+        \\ qexists_tac `ptr` \\ fs [])
+     \\ numLib.LEAST_ELIM_TAC \\ rw [] \\ fs []
+     \\ mp_then Any assume_tac IN_INFINITE_NOT_FINITE INFINITE_NUM_UNIV
+     \\ rw [] \\ pop_assum (qspec_then `domain (insert p1 ARB s.refs)` assume_tac)
+     \\ fs [FINITE_domain,domain_lookup] \\ Cases_on `lookup x (insert p1 ARB s.refs)`
+     \\ fs [] \\ qexists_tac `x` \\ Cases_on `x = p1` \\ fs [lookup_insert])
+  \\ `wf (insert p1 (ByteArray T [97w]) s.refs)` by fs [wf_insert]
+  \\ qmatch_goalsub_abbrev_tac `state_safe_for_space_fupd (K safe)  _`
+  \\ `safe` by
+     (Q.UNABBREV_TAC `safe`
+     \\ simp [data_safe_def,size_of_def,size_of_Number_head]
+     \\ fs [size_of_heap_def,stack_to_vs_def,size_of_Number_head]
+     \\ rpt (pairarg_tac \\ fs []) \\ rveq
+     \\ fs [size_of_Number_head,insert_shadow] \\ rveq
+     \\ qmatch_asmsub_abbrev_tac `closed_ptrs (a ++ b ++ c)`
+     \\ qmatch_asmsub_abbrev_tac `insert p1 x s.refs`
+     \\ qmatch_asmsub_abbrev_tac `insert p2 y (insert p1 x s.refs)`
+     \\ rveq \\ fs []
+     \\ drule size_of_insert
+     \\ disch_then (qspecl_then
+          [`b ++ c`,`LN`,`p2`,`y`,`n1''`,`refs1''`,`seen1''`] mp_tac)
+     \\ impl_tac
+     >- (fs [closed_ptrs_APPEND] \\ rw []
+        \\ ho_match_mp_tac closed_ptrs_insert \\ fs []
+        \\ Q.UNABBREV_TAC `x` \\ ho_match_mp_tac closed_ptrs_refs_insert
+        \\ fs [closed_ptrs_def])
+     \\ rw [] \\ fs []
+     \\ qpat_x_assum `wf (insert _ _ _)` kall_tac
+     \\ drule size_of_insert
+     \\ qmatch_asmsub_rename_tac `size_of (b ++ c) s.refs LN = (n8,refs8,seen8)`
+     \\ disch_then (qspecl_then [`b ++ c`,`LN`,`p1`,`x`,`n8`,`refs8`,`seen8`] mp_tac)
+     \\ impl_tac
+     >- fs [closed_ptrs_APPEND]
+     \\ rw [] \\ Cases_on `lookup ts seen1'` \\ fs [] \\ rveq
+     \\ map_every Q.UNABBREV_TAC [`x`,`y`] \\ fs [] \\ rveq
+     \\ fs [lookup_delete,lookup_insert] \\ rfs [] \\ rveq \\ fs []
+     \\ `n1' ≤ n'''''` suffices_by fs []
+     \\ ho_match_mp_tac size_of_le_APPEND
+     \\ map_every qexists_tac [`a`,`b ++ c`] \\ fs []
+     \\ asm_exists_tac \\ fs [])
+  \\ Q.UNABBREV_TAC `safe` \\ fs []
+  \\ reverse (Cases_on `call_FFI s.ffi "put_char" [97w] []` \\ fs [])
+  >- simp [data_safe_def]
+  \\ rpt (pairarg_tac \\ fs []) \\ rveq
+  \\ strip_assign \\ strip_assign
+  \\ simp [return_def,lookup_def,data_safe_def]
+  \\ rpt (pairarg_tac \\ fs [])
+  \\ rfs [insert_shadow,size_of_Number_head]
+  \\ Q.UNABBREV_TAC `rest_call`
+  (* strip tailcall *)
+  \\ ASM_REWRITE_TAC [ tailcall_def , find_code_def
+                     , get_vars_def , get_var_def
+                     , lookup_def   , timeout_def ]
+  \\ simp [code_lookup,lookup_def,lookup_insert,lookup_inter]
+  \\ IF_CASES_TAC
+  >- simp [data_safe_def]
+  \\ REWRITE_TAC [ call_env_def   , dec_clock_def
+                 , to_shallow_thm , to_shallow_def ]
+  \\ eval_goalsub_tac ``state_locals_fupd _ _``
+  \\ ho_match_mp_tac data_safe_res
+  \\ reverse conj_tac >- (rw [] \\ pairarg_tac \\ rw [])
+  \\ qmatch_goalsub_abbrev_tac `data_safe (_ s0)`
+  \\ first_x_assum (qspec_then `s0` assume_tac)
+  \\ `s0.clock < s.clock` by (UNABBREV_ALL_TAC \\ rw [])
+  \\ first_x_assum (drule_then irule) \\ Q.UNABBREV_TAC `s0` \\  fs []
+  \\ simp [ size_of_heap_def,size_of_Number_head,stack_to_vs_def
+          , lookup_def,toList_def,toListA_def
+          , wf_insert, wf_delete ]
+  \\ rw []
+  >- (pairarg_tac \\ fs []
+     \\ fs [size_of_heap_def,stack_to_vs_def,size_of_Number_head]
+     \\ rpt (pairarg_tac \\ fs []) \\ rveq
+     \\ fs [size_of_Number_head,insert_shadow] \\ rveq
+     \\ qmatch_asmsub_abbrev_tac `closed_ptrs (a ++ b ++ c)`
+     \\ qmatch_asmsub_abbrev_tac `insert p1 x s.refs`
+     \\ qmatch_asmsub_abbrev_tac `insert p2 y (insert p1 x s.refs)`
+     \\ rveq \\ fs []
+     \\ drule size_of_insert
+     \\ disch_then (qspecl_then
+          [`b ++ c`,`LN`,`p2`,`y`,`n1'`,`refs1'`,`seen1'`] mp_tac)
+     \\ impl_tac
+     >- (fs [closed_ptrs_APPEND] \\ rw []
+        \\ ho_match_mp_tac closed_ptrs_insert \\ fs []
+        \\ Q.UNABBREV_TAC `x` \\ ho_match_mp_tac closed_ptrs_refs_insert
+        \\ fs [closed_ptrs_def])
+     \\ rw [] \\ fs [size_of_def]
+     \\ rpt (pairarg_tac \\ fs []) \\ rveq \\ fs [size_of_Number_head]
+     \\ qpat_x_assum `wf (insert _ _ _)` kall_tac
+     \\ drule size_of_insert
+     \\ qmatch_asmsub_rename_tac `size_of (b ++ c) s.refs LN = (n8,refs8,seen8)`
+     \\ disch_then (qspecl_then [`b ++ c`,`LN`,`p1`,`x`,`n8`,`refs8`,`seen8`] mp_tac)
+     \\ impl_tac >- fs [closed_ptrs_APPEND]
+     \\ rveq \\ rw [] \\ Cases_on `lookup ts _` \\ fs [] \\ rveq
+     \\ map_every Q.UNABBREV_TAC [`x`,`y`] \\ fs [] \\ rveq
+     \\ fs [lookup_delete,lookup_insert] \\ rfs [] \\ rveq \\ fs []
+     \\ `n ≤ n''` suffices_by fs []
+     \\ ho_match_mp_tac size_of_le_APPEND
+     \\ map_every qexists_tac [`a`,`b ++ c`] \\ fs []
+     \\ asm_exists_tac \\ fs [])
+   \\ ho_match_mp_tac closed_ptrs_insert
+   \\ fs [] \\ reverse conj_tac
+   >- (ho_match_mp_tac closed_ptrs_refs_insert \\ fs []
+      \\ ho_match_mp_tac closed_ptrs_refs_insert \\ fs []
+      \\ fs [closed_ptrs_def])
+   \\ ho_match_mp_tac closed_ptrs_insert
+   \\ fs [] \\ reverse conj_tac
+   >- (ho_match_mp_tac closed_ptrs_refs_insert \\ fs [closed_ptrs_def])
+   \\ ONCE_REWRITE_TAC [closed_ptrs_cons]
+   \\ conj_tac >- fs [closed_ptrs_APPEND,stack_to_vs_def]
+   \\ fs [closed_ptrs_def,closed_ptrs_list_def]
   end
 QED
 
+Theorem data_safe_cyes_code_shallow[local] =
+  data_safe_cyes_code |> simp_rule [to_shallow_thm,to_shallow_def]
 
-Theorem data_safe_echo:
- ∀ffi coracle cc n. data_safe (evaluate (echo_data_call,
-                          initial_state ffi echo_data_code
+Theorem closed_ptrs_refs_compute[compute]:
+  ∀refs. closed_ptrs_refs refs =
+     EVERY (λ(k,v). case v of
+                   | ByteArray _ _ => T
+                   | ValueArray l => closed_ptrs_list l refs)
+          (toAList refs)
+Proof
+  rw [] \\ eq_tac \\ rw [closed_ptrs_refs_def]
+  >- (fs [EVERY_MEM] \\ rw [] \\ Cases_on `e`
+     \\ fs [MEM_toAList] \\ Cases_on `r` \\ fs []
+     \\ first_x_assum drule \\ fs [])
+  \\ fs [EVERY_MEM]
+  \\ first_x_assum (qspec_then `(x,ValueArray l)` assume_tac)
+  \\ fs [MEM_toAList]
+QED
+
+Theorem data_safe_cyes_code_abort:
+ ∀s ts.
+   (lookup 0 s.locals = SOME (Number 97)) ∧
+   2 ≤ s.limits.length_limit ∧
+   (s.tstamps = SOME ts) ∧
+   (s.code = cyes_data_code)
+   ⇒ ∃s' e. evaluate ((SND o SND) ^f21, s) =
+       (SOME (Rerr (Rabort e)),s')
+Proof
+  let
+    val code_lookup   = mk_code_lookup `cyes_data_code` cyes_code_def
+    val strip_assign  = mk_strip_assign code_lookup
+    val open_call     = mk_open_call code_lookup
+    val make_call     = mk_make_call open_call
+    val strip_call    = mk_strip_call open_call
+    val open_tailcall = mk_open_tailcall code_lookup
+    val make_tailcall = mk_make_tailcall open_tailcall
+  in
+  measureInduct_on `^s.clock`
+  \\ rw [to_shallow_def,to_shallow_thm]
+  \\ strip_call
+  \\ `(inter s.locals (LS ())) = LS (Number 97)`
+     by (Cases_on `s.locals` \\ fs [lookup_def,inter_def])
+  \\ strip_makespace
+  \\ ntac 6 strip_assign
+  \\ strip_call
+  \\ strip_assign
+  \\ make_if
+  \\ strip_assign
+  \\ strip_assign
+  \\ strip_assign
+  \\ strip_assign
+  (* strip_tailcall *)
+  \\ ASM_REWRITE_TAC [ tailcall_def , find_code_def
+                     , get_vars_def , get_var_def
+                     , lookup_def   , timeout_def ]
+  \\ simp [code_lookup,lookup_def,lookup_insert,lookup_inter]
+  \\ IF_CASES_TAC
+  >- simp []
+  \\ REWRITE_TAC [ call_env_def   , dec_clock_def
+                 , to_shallow_thm , to_shallow_def ]
+  \\ eval_goalsub_tac ``state_locals_fupd _ _``
+  \\ strip_assign
+  \\ make_if
+  \\ Q.UNABBREV_TAC `rest_call_1`
+  \\ strip_assign
+  \\ Q.ABBREV_TAC `pred = ∃w. 0 = w2n (w:word8)`
+  \\ `pred` by (UNABBREV_ALL_TAC \\ qexists_tac `n2w 0` \\ rw [])
+  \\ fs [] \\ pop_assum kall_tac \\ pop_assum kall_tac
+  (* strip_call *)
+  \\ qmatch_goalsub_abbrev_tac (`bind _ rest_call_1 _`)
+  \\ ONCE_REWRITE_TAC [bind_def]
+  (* open_call *)
+  \\ ASM_REWRITE_TAC [ call_def     , find_code_def , push_env_def
+                     , get_vars_def , call_env_def  , dec_clock_def
+                     , cut_env_def  , domain_def    , data_safe_def
+                     , EMPTY_SUBSET , get_var_def ]
+  \\ simp [code_lookup,lookup_def,domain_IS_SOME,lookup_insert]
+  \\ IF_CASES_TAC >- simp []
+  \\ REWRITE_TAC [ push_env_def , to_shallow_def , to_shallow_thm]
+  \\ eval_goalsub_tac ``state_locals_fupd _ _``
+  \\ strip_assign
+  \\ make_if
+  \\ strip_assign
+  \\ strip_assign
+  \\ strip_assign
+  \\ Q.ABBREV_TAC `pred = ∃w. 97 = w2n (w:word8)`
+  \\ `pred` by (UNABBREV_ALL_TAC \\ qexists_tac `n2w 97` \\ rw [])
+  \\ fs [] \\ pop_assum kall_tac \\ pop_assum kall_tac
+  \\ strip_assign
+  \\ strip_assign
+  \\ strip_assign
+  \\ strip_assign
+  (* strip_tailcall *)
+  \\ ASM_REWRITE_TAC [ tailcall_def , find_code_def
+                     , get_vars_def , get_var_def
+                     , lookup_def   , timeout_def ]
+  \\ simp [code_lookup,lookup_def,lookup_insert,lookup_inter]
+  \\ IF_CASES_TAC
+  >- simp []
+  \\ REWRITE_TAC [ call_env_def   , dec_clock_def
+                 , to_shallow_thm , to_shallow_def ]
+  \\ eval_goalsub_tac ``state_locals_fupd _ _``
+  \\ strip_assign
+  \\ make_if
+  \\ Q.UNABBREV_TAC `rest_call_1`
+  \\ ntac 3 strip_assign
+  \\ Q.ABBREV_TAC `pred = ∃w. 0 = w2n (w:word8)`
+  \\ `pred` by (UNABBREV_ALL_TAC \\ qexists_tac `n2w 0` \\ rw [])
+  \\ fs [] \\ pop_assum kall_tac \\ pop_assum kall_tac
+  \\ fs [insert_shadow]
+  \\ qmatch_goalsub_abbrev_tac `insert p2 _ (insert p1 _ s.refs)`
+  \\ `lookup p1 s.refs = NONE` by
+     (Q.UNABBREV_TAC `p1` \\ fs [least_from_def]
+     \\ EVERY_CASE_TAC \\ fs [] \\ numLib.LEAST_ELIM_TAC
+     >- metis_tac [] >- metis_tac [] >- metis_tac [] >- metis_tac []
+     \\ mp_then Any assume_tac IN_INFINITE_NOT_FINITE INFINITE_NUM_UNIV
+     \\ rw [] \\ pop_assum (qspec_then `domain s.refs` assume_tac)
+     \\ fs [FINITE_domain,domain_lookup]
+     \\ Cases_on `lookup x s.refs` \\ fs []
+     \\ asm_exists_tac \\ fs [])
+  \\ `p1 ≠ p2` by
+     (rw [Abbr `p2`,least_from_def]
+     >- (CCONTR_TAC \\ fs [])
+     >- (numLib.LEAST_ELIM_TAC \\ rw [] >- metis_tac []
+        \\ CCONTR_TAC \\ fs [lookup_insert])
+     \\ numLib.LEAST_ELIM_TAC \\ rw [] \\ fs []
+     >- (mp_then Any assume_tac IN_INFINITE_NOT_FINITE INFINITE_NUM_UNIV
+        \\ rw [] \\ pop_assum (qspec_then `domain (insert p1 ARB s.refs)` assume_tac)
+        \\ fs [FINITE_domain,domain_lookup] \\ Cases_on `lookup x (insert p1 ARB s.refs)`
+        \\ fs [] \\ qexists_tac `x` \\ Cases_on `x = p1` \\ fs [lookup_insert])
+     \\ CCONTR_TAC \\ fs [lookup_insert])
+  \\ strip_assign \\ fs [lookup_insert]
+  \\ reverse (Cases_on `call_FFI s.ffi "put_char" [97w] []`) >- simp []
+  \\ strip_assign \\ strip_assign
+  \\ rw [return_def,lookup_def]
+  \\ eval_goalsub_tac ``state_locals_fupd _ _``
+  \\ Q.UNABBREV_TAC `rest_call`
+  (*  make_tailcall *)
+  \\ ASM_REWRITE_TAC [ tailcall_def , find_code_def
+                     , get_vars_def , get_var_def
+                     , lookup_def   , timeout_def ]
+  \\ simp [code_lookup,lookup_def,lookup_insert,lookup_inter]
+  \\ IF_CASES_TAC
+  >- simp []
+  \\ eval_goalsub_tac ``call_env _ _``
+  \\ qmatch_goalsub_abbrev_tac `evaluate (p0,s0)`
+  \\ `s0.clock < s.clock` by fs [Abbr `s0`]
+  \\ first_x_assum (drule_then (qspec_then `ts + 1` mp_tac))
+  \\ impl_tac >- (fs [Abbr `s0`] \\ EVAL_TAC)
+  \\ rw [] \\ fs []
+  end
+QED
+
+Theorem data_safe_cyes_code_abort_shallow[local] =
+  data_safe_cyes_code_abort |> simp_rule [to_shallow_thm,to_shallow_def]
+
+Theorem data_safe_cyes:
+ ∀ffi coracle cc n. data_safe (evaluate (cyes_data_call,
+                          initial_state ffi cyes_data_code
                                         coracle cc T 1000 32 n))
 Proof
  let
-  val code_lookup   = mk_code_lookup `echo_data_code` echo_code_def
+  val code_lookup   = mk_code_lookup `cyes_data_code` cyes_code_def
   val strip_assign  = mk_strip_assign code_lookup
   val open_call     = mk_open_call code_lookup
   val make_call     = mk_make_call open_call
@@ -630,7 +1361,7 @@ Proof
   val open_tailcall = mk_open_tailcall code_lookup
   val make_tailcall = mk_make_tailcall open_tailcall
  in
- REWRITE_TAC [ definition "echo_data_call_def"
+ REWRITE_TAC [ definition "cyes_data_call_def"
              , to_shallow_thm
              , to_shallow_def
              , initial_state_def ]
@@ -674,19 +1405,22 @@ Proof
      (strip_makespace
      \\ ntac 7 strip_assign
      \\ make_tailcall)
-
-
-
   \\ strip_assign
-  \\ strip_call
-  \\ strip_call
-
-
-
-  let val st =
-      (snd (top_goal()) |> find_term (can (match_term ``state_locals_fupd _ _``)))
-  in EVAL ``lookup 0 ^st.locals``
+  \\ ho_match_mp_tac data_safe_bind_some
+  \\ open_call
+  \\ qmatch_goalsub_abbrev_tac `f (state_locals_fupd _ _)`
+  \\ qmatch_goalsub_abbrev_tac `f s`
+  \\ `∃s' e'. f s = (SOME (Rerr (Rabort e')),s')`
+     by (UNABBREV_ALL_TAC
+        \\ ho_match_mp_tac data_safe_cyes_code_abort_shallow
+        \\ fs [] \\ EVAL_TAC)
+  \\ `data_safe (f s)` suffices_by (rw [] \\ rfs [])
+  \\ unabbrev_all_tac
+  \\ ho_match_mp_tac data_safe_cyes_code_shallow
+  \\ rw [lookup_def,lookup_fromList,code_lookup]
+  \\ EVAL_TAC
   end
+QED
 
 val basis_pureLoop =
   let val prog = process_topdecs
@@ -700,7 +1434,7 @@ val (basis_pureLoop_call_def,basis_pureLoop_code_def) =
 
 val basis_pureLoop_ops = ops_in_prog basis_pureLoop_code_def
 
-val basis_echo =
+val basis_cyes =
   let val prog = process_topdecs `
       fun put_char c = let
         val s = String.implode [c]
@@ -714,7 +1448,7 @@ val basis_echo =
   in (rhs o concl o EVAL) ``^whole_prog ++ ^prog``
   end
 
-val basis_echo2 =
+val basis_cyes2 =
   let val prog = process_topdecs `
       fun put_char c = let
         val a = Word8Array.array 0 (Word8.fromInt 0)
@@ -728,15 +1462,15 @@ val basis_echo2 =
   in (rhs o concl o EVAL) ``^whole_prog ++ ^prog``
   end
 
-val (basis_echo_call_def,basis_echo_code_def) =
-  to_data basis_echo "basis_echo"
+val (basis_cyes_call_def,basis_cyes_code_def) =
+  to_data basis_cyes "basis_cyes"
 
-val (basis_echo2_call_def,basis_echo2_code_def) =
-  to_data basis_echo2 "basis_echo2"
+val (basis_cyes2_call_def,basis_cyes2_code_def) =
+  to_data basis_cyes2 "basis_cyes2"
 
-val basis_echo_ops = ops_in_prog basis_echo_code_def
+val basis_cyes_ops = ops_in_prog basis_cyes_code_def
 
-val bf_diff = diff_codes basis_echo_code_def basis_echo2_code_def
+val bf_diff = diff_codes basis_cyes_code_def basis_cyes2_code_def
 
 val (bf11,bf12) = hd bf_diff
 val (bf21,bf22) = (hd o tl) bf_diff
